floyd/forward_lemmas.v
@@ -367,11 +367,6 @@ Proof.
  apply H4.
 Qed.
 
-Lemma writable_share_top: writable_share Tsh.
-Admitted.
-Hint Resolve writable_share_top.
-
-
 Lemma field_mapsto_mapsto__at1:
   forall Espec Delta P Q sh ty fld e v R c Post,
     @semax Espec Delta (PROPx P (LOCALx Q (SEPx (`(field_mapsto_ sh ty fld) e :: R)))) c Post ->
